progress

Examples/AtomicCounter.v
@@ -1,23 +1,495 @@
 From LHL.Core Require Import
   Program
-  ProgramRules
   Specs
   Logic
   LogicFacts
   Tensor
   Traces
+  SingConds
+  VisPoss
+  UBLayer
+  ProgramRules
   Linearizability.
 
 From LHL.Util Require Import
-  Tactics.
+  TransUtil
+  Tactics
+  Util.
 
 From LHL.Examples Require Import
-  CounterSpec
+  RacyCounterSpec
+  AtomicCounterSpec
   LockSpec.
 
 From Coq Require Import
-  Arith.PeanoNat.
+  Logic.FunctionalExtensionality.
 
-Definition impl : Impl LockSig CounterSig :=
-  fun _ _ =>
-    .
+Definition Underlay := LockSig |+| CntSig.
+
+Definition inc : Prog Underlay unit :=
+  call Acq;;
+  call Inc;;
+  call Rel;;
+  ret tt.
+
+Definition get : Prog Underlay nat :=
+  call Acq;;
+  n <- call Get;
+  call Rel;;
+  ret n.
+
+Definition atomicCntImpl : Impl (LockSig |+| CntSig) CntSig :=
+  fun _ m => match m with
+  | Inc => inc
+  | Get => get
+  end.
+
+Definition E := Underlay.
+Definition F := CntSig.
+Definition VE T :=
+  tensorSpec (T:=T)
+    (SpecWithUB lockSpec _ LockActiveMapSound)
+    rcntSpec.
+Definition VF T := acntSpec (T:=T).
+
+Definition Relt T := SRelt (VE T) (VF T).
+Definition Prec T := SPrec (VE T) (VF T).
+
+Notation cntSt s := (RState (snd s)).
+Notation locSt s := (LState (snd s)).
+
+(*
+We start with the lock being unowned and the underlay counter equaling the overlay counter, and after R this should should still be true. We then proceed to acquiring the lock, and after R should now do nothing.
+*)
+
+Record Inv {T}
+  (s : InterState F (VE T)) (ρ : Poss (VF T))
+:= {
+  cnt_def :
+    exists k,
+      cntSt s = RCntDef (CntIdle k) /\
+      PState ρ = CntIdle k;
+  loc_def :
+    exists s',
+      locSt s = inl s'
+}.
+
+Lemma Inv_pres {T} :
+  forall s ρ t σ,
+  Inv (T:=T) s ρ ->
+  snd s = snd t ->
+  PState ρ = PState σ ->
+  Inv t σ.
+intros.
+destruct H.
+constructor.
+{
+  setoid_rewrite <- H0.
+  setoid_rewrite <- H1.
+  easy.
+}
+{ now setoid_rewrite <- H0. }
+Qed.
+
+Notation owner s := (
+  match s with
+  | LockDef o _ => o
+  end
+).
+
+Definition OwnsLock {T} (i : Name T) (s : (SpecWithUB lockSpec _ LockActiveMapSound).(State)) := (
+  exists s',
+    s = inl s' /\
+    owner s' = Some i
+).
+
+Record InvUnowned {T} (i : Name T)
+  (s : InterState F (VE T)) (ρ : Poss (VF T))
+:= {
+  unown_inv : Inv s ρ;
+  loc_unown : ~OwnsLock i (locSt s)
+}.
+
+Record InvOwned {T} (i : Name T)
+  (s : InterState F (VE T)) (ρ : Poss (VF T))
+:= {
+  own_inv : Inv s ρ;
+  loc_own : OwnsLock i (locSt s)
+}.
+
+Record Rely {T} (i : Name T)
+  (s : InterState F (VE T)) (ρ : Poss (VF T))
+  (t : InterState F (VE T)) (σ : Poss (VF T))
+:= {
+  call_pres : PCalls ρ i = PCalls σ i;
+  ret_pres : PRets ρ i = PRets σ i;
+  own_pres : InvOwned i s ρ -> InvOwned i t σ;
+  unown_pres : InvUnowned i s ρ -> InvUnowned i t σ;
+}.
+
+Definition Guar {T} (i : Name T) : Relt T :=
+  fun s ρ t σ =>
+    forall j, i <> j -> Rely j s ρ t σ.
+
+Ltac commit :=
+  unfold Commit, Guar;
+  unfold LiftSPrec, LiftSRelt;
+  unfold id; intros; do 2 psimpl.
+Ltac stable :=
+  unfold SStable, stableSPrec, stablePost, stableSRelt;
+  unfold ssub, subSRelt, subSPrec;
+  unfold Guar; intros; psimpl.
+
+Lemma eq_inj {A} :
+  forall x y : A,
+  eq x = eq y ->
+  x = y.
+intros. now rewrite H.
+Qed.
+
+Ltac eq_inj H := apply eq_inj in H; subst.
+
+Require Import Coq.Logic.Classical.
+
+Lemma not_forall {A} {P : A -> Prop} :
+  (forall x, ~P x) -> ~(exists x, P x).
+unfold not. intros. psimpl.
+now apply H with (x:=x).
+Qed.
+
+Theorem atomicCntCorrect T :
+  VerifyImpl (VE T) (VF T)
+    (fun i => LiftSRelt (Rely i))
+    (fun i => LiftSRelt (Guar i))
+    (fun i _ _ => LiftSPrec (InvUnowned i))
+    atomicCntImpl
+    (fun i _ _ _ _ _ => LiftSPrec (InvUnowned i))
+    (TReturn atomicCntImpl).
+constructor.
+{
+  unfold LiftSRelt.
+  intros. subst. exists x.
+  repeat (easy || constructor).
+}
+{
+  unfold LiftSRelt, sub, subRelt.
+  intros. psimpl.
+  specialize (H x eq_refl). psimpl.
+  specialize (H1 x2 eq_refl). psimpl.
+  exists x1. split. easy. destruct H0, H1.
+  constructor; (congruence || tauto).
+}
+{
+  unfold Guar, sub, subRelt, LiftSRelt.
+  intros. psimpl. specialize (H0 x eq_refl).
+  psimpl. exists x0. split. easy.
+  now apply H1.
+}
+{
+  unfold InvokeAny, TInvoke.
+  unfold sub, subRelt, LiftSRelt.
+  intros. psimpl. exists (invPoss i x x1).
+  split.
+  {
+    set_ext y. unfold invPoss.
+    split; intros; psimpl.
+    {
+      destruct x2, y. cbn in *.
+      f_equal.
+      { easy. }
+      {
+        extensionality k.
+        dec_eq_nats i k.
+        { now rewrite eqb_id. }
+        { now rewrite eqb_nid, H7. }
+      }
+      {
+        extensionality k.
+        dec_eq_nats i k.
+        { now rewrite eqb_id. }
+        { now rewrite eqb_nid, H8. }
+      }
+    }
+    {
+      exists x.
+      split. easy.
+      cbn. rewrite eqb_id.
+      auto using differ_pointwise_trivial.
+    }
+  }
+  {
+    assert (PState x = PState (invPoss i x x1))
+      by easy.
+    constructor; cbn.
+    { now rewrite eqb_nid. }
+    { now rewrite eqb_nid. }
+    {
+      intros. destruct H4.
+      constructor.
+      {
+        eapply Inv_pres.
+        exact own_inv0.
+        all: easy.
+      }
+      { now rewrite <- H3 at 1. }
+    }
+    {
+      intros. destruct H4.
+      constructor.
+      {
+        eapply Inv_pres.
+        exact unown_inv0.
+        all: easy.
+      }
+      { now rewrite <- H3 at 1. }
+    }
+  } 
+}
+{
+  unfold ReturnAny, TReturn.
+  unfold sub, subRelt, LiftSRelt.
+  intros. psimpl. exists (retPoss i x).
+  split.
+  {
+    set_ext y. unfold mapRetPoss, retPoss.
+    split; intros; psimpl.
+    {
+      destruct x3, y. cbn in *.
+      f_equal.
+      { easy. }
+      {
+        extensionality k.
+        dec_eq_nats i k.
+        { now rewrite eqb_id. }
+        { now rewrite eqb_nid, H8. }
+      }
+      {
+        extensionality k.
+        dec_eq_nats i k.
+        { now rewrite eqb_id. }
+        { now rewrite eqb_nid, H9. }
+      }
+    }
+    {
+      exists x.
+      split. easy.
+      cbn. rewrite eqb_id.
+      destruct H2. ddestruct H1.
+      cbn in *. symmetry in x4.
+      apply H0 in x4. specialize (x4 x3 eq_refl).
+      psimpl. repeat split; try easy.
+      apply differ_pointwise_trivial.
+      apply differ_pointwise_trivial.
+    }
+  }
+  {
+    assert (PState x = PState (retPoss i x))
+      by easy.
+    constructor; cbn.
+    { now rewrite eqb_nid. }
+    { now rewrite eqb_nid. }
+    {
+      intros. destruct H4.
+      constructor.
+      {
+        eapply Inv_pres.
+        exact own_inv0.
+        all: easy.
+      }
+      { now rewrite <- H3 at 1. }
+    }
+    {
+      intros. destruct H4.
+      constructor.
+      {
+        eapply Inv_pres.
+        exact unown_inv0.
+        all: easy.
+      }
+      { now rewrite <- H3 at 1. }
+    }
+  }
+}
+{
+  unfold LiftSPrec. intros.
+  eexists. split. easy.
+  constructor.
+  {
+    constructor.
+    { now exists 0. }
+    { now exists LockUnowned. }
+  }
+  {
+    unfold not, OwnsLock.
+    cbn. intros. psimpl.
+    now ddestruct H.
+  }
+}
+{
+  intros.
+  apply liftSPrecStable.
+  stable. now apply H0.
+}
+{
+  unfold sub, subPrec.
+  unfold LiftSRelt, LiftSPrec.
+  unfold TReturn, InterOStep.
+  intros. psimpl. ddestruct H1.
+  cbn in *. ddestruct H.
+  exists (retPoss i x3).
+  split.
+  {
+    unfold mapRetPoss, retPoss.
+    set_ext y. split; intros; psimpl.
+    {
+      destruct x5, y. cbn in *.
+      f_equal. easy.
+      {
+        extensionality j.
+        dec_eq_nats i j.
+        { now rewrite eqb_id. }
+        { now rewrite eqb_nid, H9. }
+      }
+      {
+        extensionality j.
+        dec_eq_nats i j.
+        { now rewrite eqb_id. }
+        { now rewrite eqb_nid, H10. }
+      }
+    }
+    {
+      symmetry in x2.
+      apply H0 in x2.
+      specialize (x2 x3 eq_refl).
+      psimpl. exists x3. split. easy.
+      cbn. rewrite eqb_id.
+      repeat split; try easy.
+      apply differ_pointwise_trivial.
+      apply differ_pointwise_trivial.
+    }
+  }
+  {
+    destruct H5.
+    constructor.
+    {
+      eapply Inv_pres.
+      exact unown_inv0.
+      all: easy.
+    }
+    { now rewrite <- H2 at 1. }
+  }
+}
+{
+  intros.
+  eapply weakenPrec with
+    (P:=fun _ _ => LiftSPrec (fun s x =>
+      InvUnowned i s x /\
+      Waiting i m x)).
+  2:{
+    unfold sub, subRelt, LiftSPrec, LiftSRelt.
+    unfold TInvoke. intros. psimpl.
+    specialize (H0 (invPoss i x1 m)).
+    eassert _.
+    {
+      apply H0.
+      set_ext y. unfold invPoss.
+      split; intros; psimpl.
+      {
+        destruct x0, y. cbn in *.
+        f_equal.
+        { easy. }
+        {
+          extensionality k.
+          dec_eq_nats i k.
+          { now rewrite eqb_id. }
+          { now rewrite eqb_nid, H8. }
+        }
+        {
+          extensionality k.
+          dec_eq_nats i k.
+          { now rewrite eqb_id. }
+          { now rewrite eqb_nid, H9. }
+        }
+      }
+      {
+        exists x1.
+        split. easy.
+        cbn. rewrite eqb_id.
+        auto using differ_pointwise_trivial.
+      }
+    }
+    {
+      clear H0. psimpl.
+      exists x0.
+      split.
+      { easy. }
+      split.
+      {
+        apply H0.
+        destruct H5.
+        constructor.
+        {
+          eapply Inv_pres.
+          exact unown_inv0.
+          all: easy.
+        }
+        { now rewrite <- H3 at 1. }
+      }
+      {
+        destruct H0. cbn in *.
+        rewrite eqb_id in *.
+        now constructor.
+      }
+    }
+  }
+  destruct m; cbn;
+  unfold inc, get.
+  {
+    repeat (
+      eapply lemBind;
+      intros
+    ).
+    {
+      eapply (lemCall
+        (Q:=fun _ _ => LiftSPrec (InvOwned i))
+        (S:=fun _ _ _ => LiftSPrec (InvOwned i))).
+      {
+        unfold Stable, stableRelt, sub, subRelt.
+        unfold LiftSPrec, LiftSRelt. intros. psimpl.
+        specialize (H0 x1 eq_refl). psimpl.
+        exists x0. split. easy. now apply H0.
+      }
+      {
+        unfold Stable, stablePost, stableRelt, sub, subRelt.
+        unfold LiftSPrec, LiftSRelt. intros. psimpl.
+        specialize (H0 x1 eq_refl). psimpl.
+        exists x0. split. easy. now apply H0.
+      }
+      {
+        commit.
+        exists (eq x1).
+        split.
+        { repeat econstructor. }
+        split.
+        {
+          intros. subst.
+          repeat econstructor.
+        }
+        ddestruct H; cbn in *.
+        2:{
+          exfalso. destruct H3.
+          apply not_forall in H.
+          apply H. clear H.
+          unfold OwnsLock in loc_unown0.
+          destruct s, s, LState; cbn in *.
+          2: easy. destruct s. cbn in *.
+          ddestruct x2.
+        }
+        2:{
+          destruct H3, unown_inv0.
+          psimpl. now rewrite H3 in x2.
+        }
+      }
+    }
+  }
+}
