Examples/RacyCounterSpec.v
@@ -1,0 +1,29 @@
+From LHL.Core Require Import
+  Program
+  Specs.
+
+From LHL.Examples Require Import
+  AtomicCounterSpec.
+
+Variant RacyCntState {T} :=
+| RCntDef (s : CntState T)
+| RCntUB (m : ActiveMap T CntSig).
+Arguments RacyCntState : clear implicits.
+
+Variant RacyCntStep {T} : RacyCntState T -> ThreadEvent T CntSig -> RacyCntState T -> Prop :=
+| DefStep s e t :
+  cntPend s = None ->
+  CntStep s e t ->
+  RacyCntStep (RCntDef s) e (RCntDef t)
+| UBStep s i A (m : CntSig A) t :
+  cntPend s <> None ->
+  RacyCntStep (RCntDef s) (i, CallEv m) (RCntDef t).
+
+Program Definition rcntSpec {T} : Spec T CntSig := {|
+  State := RacyCntState T;
+  Init := RCntDef acntSpec.(Init);
+  Step := RacyCntStep
+|}.
+
+Next Obligation.
+Admitted.
